@prefix owl: <http://www.w3.org/2002/07/owl#> .
@prefix xsd: <http://www.w3.org/2001/XMLSchema#> .
@prefix dc: <http://purl.org/dc/terms/> .
@prefix rdfs: <http://www.w3.org/2000/01/rdf-schema#> .
@prefix rdf: <http://www.w3.org/1999/02/22-rdf-syntax-ns#> .
@prefix eeboo: <http://eeboo.oerc.ox.ac.uk/eeboo/> .
@prefix bf: <http://bibframe.org/vocab/> .
@prefix mads: <http://www.loc.gov/mads/rdf/v1#> .
@prefix mods: <http://www.loc.gov/mods/v3#> .

<http://eeboo.oerc.ox.ac.uk/eeboo>
  a owl:Ontology .
  
# Classes 
  
eeboo:Person
    a rdfs:Class ;
    rdfs:label "Person" ;
    owl:equivalentClass bf:Person ;
    rdfs:comment "A human being" .

eeboo:Work
    a rdfs:Class ;
    rdfs:label "Work" ;
	owl:equivalentProperty bf:Instance ;
    rdfs:comment "A physical thing, the metadata details of which are captured in an object record such as an EEBO xml-file" .

eeboo:Surname
    a rdfs:Class ;
    rdfs:label  "Surname" ;
    owl:equivalentClass mads:FamilyNameElement ;
    rdfs:comment "Surname or Family name of a person, i.e. the name shared by members of the same family, e.g. Smith" .

eeboo:Personal_Name
    a rdfs:Class ;
    rdfs:label  "FirstName" ;
    owl:equivalentClass mads:GivenNameElement ;
    rdfs:comment "Given, personal name of an individual person, usually the name they are referred to by friends and family, e.g. John" .


#Properties
eeboo:raw_pubplace
  a rdf:Property, owl:DatatypeProperty ;
  rdfs:domain eeboo:Work ;
  rdfs:range xsd:string .

eeboo:precise-birth
  a rdf:Property, owl:DatatypeProperty ;
  rdfs:comment "The birth date of a person when it has been recorded without ambiguity or uncertainty" ;
  rdfs:domain eeboo:Person ;
  rdfs:label  "precise-date-of-birth"^^xsd:string;
  rdfs:range xsd:date .

eeboo:precise-death
    a rdf:Property, owl:DatatypeProperty ;
    rdfs:comment "The date of death of a person when it has been recorded without ambiguity or uncertainty" ;
    rdfs:domain eeboo:Person ;
    rdfs:label  "precise-date-of-death"^^xsd:string;
    rdfs:range xsd:date .
	
eeboo:approximate-birth
    a rdf:Property, owl:DatatypeProperty ;
    rdfs:comment "The birth date of a person when it has been recorded ambiguously or with a degree of uncertainty" ;
    rdfs:domain eeboo:Person ;
    rdfs:label  "approximate-date-of-birth"^^xsd:string;
    rdfs:range xsd:date .
  
eeboo:approximate-death
      a rdf:Property, owl:DatatypeProperty ;
      rdfs:comment "The date of death of a person when it has been recorded ambiguously or with a degree of uncertainty" ;
      rdfs:domain eeboo:Person ;
      rdfs:label  "approximate-date-of-death"^^xsd:string;
      rdfs:range xsd:date .
	  
eeboo:precise-floruit-start
      a rdf:Property, owl:DatatypeProperty ;
      rdfs:comment "The start date of a period of professional activity for a person when that time range has been recorded without ambiguity or uncertainty" ;
      rdfs:domain eeboo:Person ;
      rdfs:label  "precise-floruit-start"^^xsd:string;
      rdfs:range xsd:date .
	  
eeboo:precise-floruit-end
      a rdf:Property, owl:DatatypeProperty ;
      rdfs:comment "The end date of a period of professional activity for a person when that time range has been recorded without ambiguity or uncertainty" ;
      rdfs:domain eeboo:Person ;
      rdfs:label  "precise-floruit-end"^^xsd:string;
      rdfs:range xsd:date .
	  
eeboo:precise-publication
    a rdf:Property, owl:DatatypeProperty ;
    rdfs:comment "The publication date of a work when it has been recorded without ambiguity or uncertainty" ;
    rdfs:domain eeboo:Work ;
    rdfs:label  "precise-publication"^^xsd:string;
    rdfs:range xsd:date .
  
eeboo:approx-publication
    a rdf:Property, owl:DatatypeProperty ;
    rdfs:comment "The approximate publication date of a work i.e. when it has been recorded with ambiguity or uncertainty" ;
    rdfs:domain eeboo:Work ;
    rdfs:label  "precise-publication"^^xsd:string;
    rdfs:range xsd:date .

eeboo:surname
  a rdf:Property ;
  rdfs:domain eeboo:Person ;
  rdfs:label  "has_surname" ;
  rdfs:range eeboo:Surname .

eeboo:given_name
  a rdf:Property ;
  rdfs:domain eeboo:Person ;
  rdfs:label  "has_personal_name" ;
  rdfs:range eeboo:Personal_Name .

eeboo:creator
    a rdf:Property ;
    rdfs:domain eeboo:Work ;
    rdfs:label  "has_creator" ;
    owl:equivalentProperty dc:creator ;
    rdfs:range eeboo:Person .
	
eeboo:electronicLocation
	a rdf:Property ;
	rdfs:domain eeboo:Work ;
	rdfs:label  "electronic_representation_of_resource" ;
	rdfs:range xsd:string .

eeboo:hasExternalAuthorityVIAF
	a rdf:Property ;
	rdfs:domain eeboo:Person ;
	rdf:subPropertyOf mads:hasExactExternalAuthority ;
	rdfs:label  "Records the uri of the exact match entitity from VIAF" ;
	rdfs:range xsd:string .

eeboo:hasExternalAuthorityLoC
	a rdf:Property ;
	rdfs:domain eeboo:Person ;
	rdf:subPropertyOf mads:hasExactExternalAuthority ;
	rdfs:label  "Records the uri of the exact match entitity from Library of Congress" ;
	rdfs:range xsd:string .
	
	
	


